I don't know what I did but I got something!

src/monad.lean
@@ -1,31 +1,79 @@
 import Mathlib.Data.Nat.Basic
 
+open Std.Range Std.Range.forIn
+
 def ff (n : ℕ) : ℕ := Id.run do
   let mut r := 0
   for _ in [: n] do
     r ← r + 1
   return r
 
+variable {m : Type u → Type v} [Monad m]
+
+def mkRange (start stop step : ℕ) : Std.Range := { start := start, stop := stop, step := step }
+
+def mkRange' (start stop : ℕ) : Std.Range := { start := start, stop := stop, step := 1 }
+
+def extractStep (s : ForInStep β) : m β :=
+  match s with
+    | ForInStep.done b => pure b
+    | ForInStep.yield b => pure b
+
 -- For a function that's independent of the loop variable
 -- The result only depends on the number of iterations
 -- Notes: In `f i r`, `i` is the loop variable and `r` is the "program state"
--- Notes: `Std.Range.forIn.loop f fuel i stop step b`
-theorem succ_invariant {β : Type u} {m : Type u → Type v} {b : β} [Monad m]
-(f : ℕ → β → m (ForInStep β)) (hf : ∀ i j : ℕ, f i = f j) :
-  Std.Range.forIn.loop f k 0 k 1 b = Std.Range.forIn.loop f k 1 (k + 1) 1 b := by
+-- Notes: `Std.Range.forIn range init f`
+theorem succ_invariant {k : ℕ} {init : β} {f : ℕ → β → m (ForInStep β)}
+  (hf : ∀ i j : ℕ, f i = f j) :
+  Std.Range.forIn (mkRange' 0 k) init f
+  = Std.Range.forIn (mkRange' 1 k.succ) init f := by
+  sorry
+
+-- We can decompose a for loop range into two parts and execute them separately
+-- Only succ is specified here
+theorem range_decompose {start mid stop : ℕ} :
+  Std.Range.forIn (mkRange' start stop) init f =
+    Std.Range.forIn (mkRange' mid stop) (Id.run (Std.Range.forIn (mkRange' start mid) init f)) f := by
   sorry
 
 def incStep : ℕ → ℕ → Id (ForInStep ℕ) := λ _ r => ForInStep.yield (r + 1)
 
+-- set_option pp.all true
+
+-- Interesting technicality - since the definition of `loop` depends on 0 < fuel, we have to cases
+theorem emptyStep' {k : ℕ} {init : β} {f : ℕ → β → Id (ForInStep β)} :
+  loop f fuel k k 1 init = init := by
+    cases k <;> cases fuel <;> simp [loop]
+
+theorem emptyStep {k : ℕ} {init : β} {f : ℕ → β → Id (ForInStep β)} :
+  Std.Range.forIn (mkRange' k k) init f = init := emptyStep'
+
+theorem singleIncStep {k : ℕ} : Std.Range.forIn (mkRange' k k.succ) init incStep = init + 1 := by
+  simp [mkRange', Std.Range.forIn, loop, incStep, Nat.succ_eq_add_one,
+        show (Nat.succ k ≤ k) = False by simp]
+  exact emptyStep'
+
+theorem incStep_succ_invariant : ∀ i j : ℕ, incStep i = incStep j := by simp [incStep]
+
 -- This is kind of an ad-hoc theorem for the simple program
 -- Also, I have a question: `s` is a Nat here and the loop (RHS) is a `Id Nat`
 -- How do they compare?
-theorem state_invariant {s : ℕ} (h : s = Std.Range.forIn.loop incStep k 0 k 1 0) :
-  s + 1 = Std.Range.forIn.loop incStep k 0 k 1 1 := by
-  sorry
+theorem state_invariant {n : ℕ} (init : ℕ) :
+  Id.run (Std.Range.forIn (mkRange' 0 n) init incStep) + 1
+  = Std.Range.forIn (mkRange' 0 n.succ) init incStep := by
+  induction' n with k hk
+  -- n = 0
+  simp [Id.run, Std.Range.forIn, incStep, loop]
+  -- n = k → n = k + 1
+  simp [Id.run] at *
+  rw [@range_decompose _ _ _ _ k.succ k.succ.succ, Id.run, ← hk, singleIncStep]
 
 theorem ff' : ff n = n := by
   induction' n with k hk
   simp
-  simp [ff, Id.run, forIn, Std.Range.forIn, Std.Range.forIn.loop, ← succ_invariant] at *
-  exact (state_invariant hk.symm).symm
+  let h := (@state_invariant k 0)
+  simp [ff, Id.run, forIn, Std.Range.forIn, loop, ← succ_invariant] at *
+  simp [Id.run, incStep, mkRange', Std.Range.forIn] at h
+  conv_rhs => rw [← hk, Nat.succ_eq_add_one, h]
+
+example : ff 5 = 5 := ff'
